DP_CRelVS.thy
@@ -242,7 +242,43 @@ proof -
   show ?thesis
     unfolding fold\<^sub>T_def by transfer_prover
 qed
+  
+definition "KK R P x y \<equiv> R x y \<and> P x"
+  
+lemma map_transfer':
+  fixes R0 R1 xs xs\<^sub>T' f f\<^sub>T'
+  assumes "list_all2 (KK R0 (\<lambda>x. x\<in>set xs)) xs xs\<^sub>T'"
+  assumes "((KK R0 (\<lambda>x. x\<in>set xs)) ===> crel_vs R1) f f\<^sub>T'"
+  shows "crel_vs (list_all2 R1) (map f xs) (map\<^sub>T' f\<^sub>T' xs\<^sub>T')"
+    using assms(1)
+    apply (induction rule: list_all2_induct; unfold list.map map\<^sub>T'.simps)
+    subgoal premises prems[transfer_rule] by transfer_prover
+    subgoal premises prems[transfer_rule] supply [transfer_rule] = assms(2) by transfer_prover
+    done
+      
+lemma [transfer_rule]:
+  assumes "list_all2 R xs xs\<^sub>T'"
+  shows "list_all2 (KK R (\<lambda>x. x\<in>set xs)) xs xs\<^sub>T'"
+  using assms
+  unfolding list_all2_iff
+  unfolding KK_def
+  unfolding set_zip
+  by auto
 
+notepad
+begin
+  fix R0::"'a \<Rightarrow> 'b \<Rightarrow> bool" and R1::"'a \<Rightarrow> 'b \<Rightarrow> bool" and R::"'a \<Rightarrow> 'b \<Rightarrow> bool" and f g
+  assume fg: "(R0 ===> R1) f g"
+  assume rr: "\<And>x y. R x y \<Longrightarrow> R0 x y"
+  fix a b
+  assume ab: "R a b"
+  have "R1 (f a) (g b)"
+    supply [transfer_rule] = fg rr ab
+    apply transfer_prover_start
+      apply transfer_step
+     back
+      apply transfer_step
 end
 end
+  
 end
